theories/examples/authentikit_susp_security.v
@@ -14,32 +14,245 @@ Definition table_inv `{!invGS_gen hlc Σ} `{!tableG Σ} (N : namespace) (P : iPr
   na_inv tableG_name N P.
 Definition table_tok `{!invGS_gen hlc Σ} `{!tableG Σ} (E : coPset) :=
   na_own tableG_name E. *)
-
+  
 Section proof.
-  Context `{!authG Σ, !seqG Σ}.
+  Context `{!stateG Σ, !authG Σ, !seqG Σ}.
 
   Definition authBaseN : namespace := nroot .@ "susp_ver".
   Definition authN (v : val) : namespace := authBaseN .@ v.
+  Definition gmapN : namespace := authBaseN .@ "gmap".
   Definition tableN : namespace := authBaseN .@ "table".
+  Definition tableLocSet : namespace := authBaseN .@ "tableloc".
+  Definition tableLocN (susp : val) : namespace := tableLocSet .@ susp.
 
   Definition lrel_auth := lrel_auth authBaseN.
 
-  Definition finish_spec (A : lrel Σ) (finish : val) (t : evi_type) (x a2 : val) : iProp Σ :=
-    {{{ seq_tok ⊤ }}}
+  (* Definition proph_type : Type := nat * option unit.
+
+  Definition proph_cond (v : proph_type) (pid : nat) : iProp Σ :=
+    (∀ (m : parentUR), ∃ (x av : val) (t : evi_type),
+        ⌜v = (pid, Some tt)⌝ ∗ val_eq t x av ∗
+          ⌜m !! pid = Some (to_agree (t, x))⌝) ∨
+      (⌜v = (pid, None)⌝).
+
+  Fixpoint take_until {A B : Type} (f : A → option B) (xs : list A) : list B :=
+    match xs with
+    | []      => []
+    | x :: xs =>
+      match f x with
+      | Some y => y :: (take_until f xs)
+      | None   => []
+      end
+    end.
+
+  Definition longest_valid_prefix (us : list val) : list proph_type :=
+    take_until (λ u,
+        match u with
+          (#(LitInt v), SOMEV #())%V => if Z.geb v 0 then Some (Z.to_nat v, Some ()) else None
+        | (#(LitInt v), NONEV)%V => if Z.geb v 0 then Some (Z.to_nat v, None) else None
+        | _ => None
+        end
+      ) us.
+
+  Definition proph_list (p : proph_id) (vs : list (nat * option unit)) : iProp Σ :=
+    ∃ (us : list (val * val)),
+      proph p us ∗ ⌜vs = longest_valid_prefix (map snd us)⌝
+        ∗ [∗ list] k↦v ∈ vs, (∃ (pid : nat), proph_cond v pid).
+
+  Definition option_unit_val (v : option unit) : val :=
+    match v with Some _ => SOMEV #() | None => NONEV end.
+  
+  Lemma wp_resolve_proph_val_some p vs (pid : nat) :
+    ∀ x av t (m : parentUR),
+      {{{ proph_list p vs ∗ val_eq t x av ∗ ⌜m !! pid = Some (to_agree (t, x))⌝ }}}
+        resolve_proph: #p to: (#pid, SOMEV #())%V
+      {{{ vs', RET #(); ⌜vs = (pid, Some tt) :: vs'⌝ ∗ proph_list p vs' }}}.
+  Proof.
+    iIntros (???? Φ) "((%us & Hp & % & Hcon) & Heq & %Hmap) HΦ".
+    wp_apply (wp_resolve_proph with "Hp").
+    iIntros (us') "[% Hp]". simplify_eq.
+    iApply "HΦ". iFrame "Hp". iSplit; [|iSplit; [done|]].
+    - iPureIntro. simpl.
+      rewrite /longest_valid_prefix. simpl.
+      assert ((pid >=? 0)%Z = true).
+      { rewrite Z.geb_le. lia. }
+      rewrite H. do 2 f_equal. lia.
+    - iSimpl in "Hcon".
+      rewrite /longest_valid_prefix.
+      assert ((pid >=? 0)%Z = true).
+      { rewrite Z.geb_le. lia. }
+      simpl. rewrite H. simpl.
+      iDestruct "Hcon" as "[H1 Hcon]". iFrame.
+  Qed.
+  
+  Lemma wp_resolve_proph_val_none p vs (pid : nat) :
+    {{{ proph_list p vs }}}
+      resolve_proph: #p to: (#pid, NONEV)%V;;
+      resolve_proph: #p to: NONEV
+    {{{ RET #(); ⌜vs = [(pid, None)]⌝ }}}.
+  Proof.
+    iIntros (Φ) "(%us & Hp & %) HΦ".
+    wp_apply (wp_resolve_proph with "Hp").
+    iIntros (?) "[% Hp]". wp_pures.
+    wp_apply (wp_resolve_proph with "Hp").
+    iIntros (?) "[% Hp]". iApply "HΦ".
+    simplify_eq. iPureIntro.
+    rewrite /longest_valid_prefix /option_unit_val.
+    simpl; f_equal.
+    assert ((pid >=? 0)%Z = true).
+    { rewrite Z.geb_le. lia. }
+    rewrite H. do 2 f_equal. lia.
+  Qed.
+
+  Lemma wp_resolve_proph_final p vs (v : option unit) :
+    {{{ proph_list p vs }}}
+      resolve_proph: #p to: (#0, option_unit_val v)%V;;
+      resolve_proph: #p to: NONEV
+    {{{ RET #(); ⌜vs = [(0, v)]⌝ }}}.
+  Proof.
+    iIntros (Φ) "(%us & Hp & %) HΦ".
+    wp_apply (wp_resolve_proph with "Hp").
+    iIntros (?) "[% Hp]". wp_pures.
+    wp_apply (wp_resolve_proph with "Hp").
+    iIntros (?) "[% Hp]". iApply "HΦ".
+    simplify_eq. iPureIntro.
+    rewrite /longest_valid_prefix /option_unit_val.
+    destruct v; simpl; [destruct u|]; f_equal.
+  Qed. *)
+
+  Definition finish_spec1 (finish : val) (x a aᵥ aᵢ ser : val) (A : lrel Σ) : iProp Σ :=
+    ∀ (s : string) (E: coPset) (t1 t2 : evi_type),
+      ⌜↑authSerProofSet authBaseN ⊆ E⌝ -∗
+      {{{ seq_tok E ∗ count_is_correct t1 x 0 ∗ A aᵥ aᵢ ∗
+            ser_spec_3 ser t1 ∗ val_eq_rel authBaseN A t1 ∗ hashed s ∗
+            s_is_ser'' t2 aᵥ s ∗ ⌜a = InjLV #(hash s)⌝ }}}
         finish #()
-    {{{ (o : option val), RET $o; seq_tok ⊤ ∗
-                                    if o is None then ⌜True⌝ else
-                                      (∃ (a1 : val), A a1 a2 ∗ val_eq t x a1) }}}.
-        
+        {{{ (o : option val), RET $o;
+            seq_tok E ∗ if o is None then True else A x aᵢ }}}.
+
+  Definition finish_spec2 (finish : val) (x a aᵥ aᵢ ser : val) (A : lrel Σ) : iProp Σ :=
+    ∀ (s1 s2 : string) (E: coPset) (susp : loc) (t1 t2 : evi_type),
+      {{{ seq_tok E ∗ count_is_correct t1 x 0 ∗ A aᵥ aᵢ ∗
+            ser_spec_3 ser t1 ∗ val_eq_rel authBaseN A t1 ∗ hashed s2 ∗
+            s_is_ser'' t2 aᵥ s1 ∗ ⌜a = InjRV #susp⌝ ∗ susp ↦□ InjRV #(hash s2) }}}
+        finish #()
+        {{{ (o : option val), RET $o;
+            seq_tok E ∗ if o is None then True else ⌜s1 = s2⌝ -∗ val_eq t1 x aᵥ }}}.
+
+  (* Definition finish_spec (finish : val) (t : evi_type) (x : val) : iProp Σ :=
+    ∀ (E : coPset) (ser av ai : val),
+      ⌜↑authSerProofSet authBaseN ⊆ E⌝ -∗ ⌜↑tableN ⊆ E⌝ -∗ ⌜↑tableLocSet ⊆ E⌝ -∗
+      {{{ A av ai ∗ ser_spec_3 ser t ∗ seq_tok E ∗ count_is_correct t x 0 }}}
+        finish #() @ E
+        {{{ (o : option val), RET $o;
+            seq_tok E ∗ if o is None then ⌜True⌝ else
+                (A x ai ∗ val_eq t x av) }}}. *)
+
+  Definition susp_big_sep (m : gmap val val) : iProp Σ :=
+    [∗ map] k ↦ v ∈ m,
+      ∃ (id ctr : nat) (finish ctrv x a aᵥ aᵢ ser : val) (t : evi_type) (A : lrel Σ) (b : bool),
+        (⌜k = #id ∧ ctrv = #ctr ∧ ctr > 0 ∧ v = (ctrv, finish)%V⌝ ∗ A aᵥ aᵢ ∗
+           count_is_correct t x ctr ∗ single_instance id t x aᵥ None b ∗
+           (∃ (h: string), (⌜a = InjLV #h⌝ ∗ finish_spec1 finish x a aᵥ aᵢ ser A) ∨
+                             (∃ (susp : loc), ⌜a = InjRV #susp⌝ ∗ susp↦□ InjRV #h ∗
+                                                finish_spec2 finish x a aᵥ aᵢ ser A))).
+      
   Definition is_susp_table (l : loc) : iProp Σ :=
+    ∃ (d : val) (m : gmap val val),  l ↦ d ∗ ⌜is_map d m⌝ ∗ susp_big_sep m.
+
+  Definition in_susp_table (l : loc) (id : nat) : iProp Σ :=
+    ∃ (d v : val) (m : gmap val val),
+      is_susp_table l -∗ l ↦ d ∗ ⌜is_map d m⌝
+      -∗ is_susp_table l ∗ ⌜m !! #id = Some v⌝.
+
+  Definition not_in_susp_table (l : loc) (id : nat) : iProp Σ :=
     ∃ (d : val) (m : gmap val val),
-      l ↦ d ∗ ⌜is_map d m⌝ ∗
-        ([∗ map] k ↦ v ∈ m, ∃ (pid ctr : nat) (finish ctrv : val) (A : lrel Σ),
-            (⌜k = #pid ∧ ctrv = #ctr ∧ ctr > 0 ∧ v = (ctrv, finish)%V⌝ ∗
-               (∃ (t: evi_type) (x a2 : val), finish_spec A finish t x a2))).
+      is_susp_table l -∗ l ↦ d ∗ ⌜is_map d m⌝
+      -∗ is_susp_table l ∗ ⌜m !! #id = None⌝.
 
   Definition inv_susp_table (l: loc) := seq_inv tableN (is_susp_table l).
 
+  Definition count_inv (cnt : nat) (m : mapUR) (lm : locPidMapUR) :=
+    ∀ (id : nat),
+      id ≥ cnt →
+      (m !! id = None ∧
+         (∀ (l : loc), lm !! l = None ∨
+                         (∀ id', lm !! l = Some id' → id ≠ id'))).
+  
+  Definition global_state (cnt : nat) (m : mapUR) (lm : locPidMapUR) : iProp Σ :=
+    own stateG_name (● (MaxNat (cnt-1), m, lm)) ∗
+      ⌜count_inv cnt m lm⌝ ∗
+      (∀ (id : nat) (x vᵥ : val) (l : loc) (t : evi_type),
+          ⌜m !! id = Some (to_agree (t, x, vᵥ, (None : option loc), true))⌝ ∗
+            (in_susp_table l id ∨ (not_in_susp_table l id ∗ val_eq t x vᵥ))).
+  
+  Definition empty_state n : prodUR (prodUR max_natUR mapUR) locPidMapUR := (MaxNat n, ∅, ∅).
+  
+  Lemma global_state_update_empty E (cnt : nat) (m : mapUR) (lm : locPidMapUR) :
+    global_state cnt m lm ={E}=∗ global_state (cnt + 1) m lm.
+  Proof.
+    iIntros "(Hproph & %Hcntinv & Hseminv)".
+    iMod ((own_update
+             stateG_name
+             (● (MaxNat (cnt-1), m, lm))
+             (● (MaxNat cnt, m, lm) ⋅ ◯ (empty_state cnt) ))
+           with "Hproph") as "Hproph".
+    { apply (auth_update _ (empty_state 0) _ _).
+      do 2 apply prod_local_update_1.
+      apply max_nat_local_update.
+      simpl. lia. }
+    iPoseProof (own_op with "Hproph") as "[Hproph _]".
+    iModIntro. rewrite /global_state.
+    rewrite Nat.add_sub. iFrame. iPureIntro.
+    intros id H. apply Hcntinv. lia.
+  Qed.
+
+  Definition singleton_map (id : nat) (t : evi_type) (x vᵥ : val) (so : option loc) (b : bool) : mapUR :=
+    {[ id := to_agree (t, x, vᵥ, so, b) ]}.
+
+  Definition single_instance_frag (id : nat) (t : evi_type) (x vᵥ : val) (so : option loc) (b : bool) : stateUR :=
+    ◯ (MaxNat id, singleton_map id t x vᵥ so b, if so is Some s then {[ s := id ]} else ∅).
+
+  Definition updated_map (m : mapUR) (id : nat) (t : evi_type) (x vᵥ : val) (so : option loc) (b : bool) : mapUR :=
+    <[ id := to_agree (t, x, vᵥ, so, b) ]> m.
+
+  Definition updated_loc_map (m : locPidMapUR) (so : option loc) (id : nat) : locPidMapUR :=
+    if so is Some s then <[ s := id ]> m else m.
+
+  Lemma global_state_update_singleton E (cnt : nat) (m : mapUR) (lm : locPidMapUR) (t : evi_type) (x vᵥ : val) (so : option loc) (b : bool) :
+    global_state cnt m lm
+    ={E}=∗ global_state (cnt + 1) (updated_map m cnt t x vᵥ so b) (updated_loc_map lm so cnt) ∗ single_instance cnt t x vᵥ so b.
+  Proof.
+    iIntros "(Hproph & %Hcntinv & Hseminv)".
+    iMod ((own_update
+             stateG_name
+             (● (MaxNat (cnt-1), m, lm))
+             (● (MaxNat cnt, updated_map m cnt t x vᵥ so b, updated_loc_map lm so cnt) ⋅ single_instance_frag cnt t x vᵥ so b))
+           with "Hproph") as "Hproph".
+    { apply (auth_update _ (empty_state 0) _ _).
+      apply prod_local_update; simpl.
+      { apply prod_local_update; simpl.
+        { apply max_nat_local_update. simpl. lia. }
+        apply gmap.alloc_local_update; last done.
+        apply Hcntinv. lia. }
+      destruct so; last done.
+      admit. }
+    iPoseProof (own_op with "Hproph") as "[Hproph Hfrag]".
+    iModIntro. rewrite /global_state.
+    rewrite Nat.add_sub. iFrame. iSplitR "Hseminv".
+    iPureIntro.
+    { intros id H. rewrite /updated_map.
+      rewrite lookup_insert_None.
+      split; last admit.
+      split; last lia.
+      apply Hcntinv. lia. }
+    iIntros (?????).
+    iSpecialize ("Hseminv" $! id x0 vᵥ0 l t0) as #.
+    iDestruct "Hseminv" as "[%Hseminv $]".
+    iPureIntro. unfold updated_map.
+  Admitted.
+  
+    
 (*  Definition proph_list (vs : val) : iProp Σ :=
     ∃ (m: gmap int proph_id),
       ([∗ map] id ↦ p ∈ m, ∃ ( 
@@ -52,44 +265,191 @@ Section proof.
       resolves pid -∗ is_fine A 
     else
       .*)
-  
-  Lemma v_finish_spec (A : lrel Σ) :
-    ∀ (st : loc) (a a1 a2 x ser : val) (t : evi_type) (c : nat) (h : string),
-      inv_susp_table st ⊢
-      {{{ (lrel_auth A) a a2 ∗ ⌜a = SOMEV a1 ∧ a1 = InjLV #h⌝ ∗ seq_tok ⊤ ∗
-            ser_spec_3 authBaseN ser t ∗ count_is_correct authBaseN t x c
-            (* (∃ (p: proph_id) (vs : list (val * val)), ⌜pv = #p⌝ ∗ proph p vs)*) }}}
-        v_finish #st a1 x ser
-      {{{ (finish : val), RET finish;
-          finish_spec A finish t x a2 ∗ seq_tok ⊤ }}}.
+
+  Lemma v_finish_spec1 :
+    ∀ (a aᵥ aᵢ x ser : val) (st : loc) (A : lrel Σ),
+      {{{ inv_susp_table st }}}
+        v_finish #st a x ser
+        {{{ (finish : val), RET finish;
+            finish_spec1 finish x a aᵥ aᵢ ser A }}}.
   Proof.
-    iIntros (?????????) "#Htab".
-    iIntros (?) "!# (#Hauth & (-> & ->) & Htok & #Hserspec & #Hcount) HΦ".
+    iIntros (????????) "#Htab HΦ".
     rewrite /v_finish.
-    iDestruct "Hauth" as "[(% & % & Hauth)|%]"; [|done].
+    wp_pures. iModIntro. iApply "HΦ".
+    rewrite /finish_spec1.
+    iIntros (?????).
+    iIntros (?) "!# (Htok & Hcount & #HA & #Hserspec & #Hrel & #hashs & #Hser & %) HΦ".
+    wp_pures. wp_apply ("Hserspec" with "[$Hcount $Htok]").
+    iIntros ([]); last first.
+    { iIntros "(Htok & #Hsers)". wp_pures.
+      iModIntro. iApply ("HΦ" $! None). eauto. }
+    iIntros "(Htok & #Hsers)". wp_pures.
+    simplify_eq. wp_pures.
+    wp_apply (wp_hash); try done.
+    iIntros "#hashs0". wp_pures.
+    case_bool_decide; simplify_eq; wp_pures;
+      try ( iApply ("HΦ" $! None); eauto ).
+
+    destruct (decide (collision s s0)) as [|Hnc%not_collision];
+      try (iExFalso; by iApply (hashes_auth.hashed_inj_or_coll with "hashs hashs0") ).
+    destruct Hnc as [<-|?]; simplify_eq.
+    iPoseProof (evi_type_ser''_inj authBaseN with "[Hsers] Hser") as "Heq";
+      try (iLeft; iFrame "#").
+    iApply ("HΦ" $! (Some _)).
+    iPoseProof (val_eq_sym authBaseN with "Heq") as "Heq1".
+    iMod ("Hrel" with "[] [Htok]") as "(Htok & Heq2)";
+      iFrame "∗ #"; try done.
+  Qed.
+    
+  Lemma v_finish_spec2 :
+    ∀ (a x aᵥ aᵢ ser : val) (st : loc) (A : lrel Σ),
+      {{{ inv_susp_table st }}}
+        v_finish #st a x ser 
+      {{{ (finish : val), RET finish;
+          finish_spec2 finish x a aᵥ aᵢ ser A }}}.
+  Proof.
+    iIntros (????????) "#Htab HΦ".
+    rewrite /v_finish.
+    wp_pures. iModIntro. iApply "HΦ".
+    rewrite /finish_spec2.
+    iIntros (?????).
+    iIntros (??) "!# (Htok & Hcount & #HA & #Hserspec & #Hrel & #hashs2 & #Hser & % & #Hsusp) HΦ".
+    wp_pures. wp_apply ("Hserspec" with "[$Hcount $Htok]").
+    iIntros ([]); last first.
+    { iIntros "(Htok & #Hsers)". wp_pures.
+      iModIntro. iApply ("HΦ" $! None). eauto. }
+    iIntros "(Htok & #Hsers)". wp_pures.
+    simplify_eq. wp_pures. wp_load. wp_pures.
+    wp_apply (wp_hash); try done.
+    iIntros "#hashs". wp_pures.
+    case_bool_decide; simplify_eq; wp_pures;
+      try ( iApply ("HΦ" $! None); eauto ).
+
+    destruct (decide (collision s s2)) as [|Hnc%not_collision];
+      try (iExFalso; by iApply (hashes_auth.hashed_inj_or_coll with "hashs hashs2") ).
+    destruct Hnc as [<-|?]; simplify_eq.
+    iApply ("HΦ" $! (Some _)).
+    iFrame.
+    iModIntro. iIntros (->).
+    iApply (evi_type_ser''_inj authBaseN); [by iLeft|done].
+  Qed.
+
+  (* Lemma v_finish_spec_2 :
+    ∀ (st : loc) (a a1 a2 x ser : val) (t : evi_type) (pid: nat) (susp : loc) (E : coPset) (A : lrel Σ),      
+      inv_susp_table st ⊢
+        {{{ ⌜a = InjRV #susp⌝ ∗ susp ↦ InjLV #pid ∗
+              ser_spec_3 ser t ∗ A a1 a2 }}}
+        v_finish #st a x ser @ E
+        {{{ (finish : val), RET finish;
+            finish_spec2 finish t x }}}.
+  Proof.
+    iIntros (???????????) "#Htab".
+    iIntros (?) "!# (% & Hsusp & #Hserspec & #HA) HΦ".
+    rewrite /v_finish.
     simplify_eq. wp_pures. iModIntro.
     iApply "HΦ". iFrame.
-    rewrite /finish_spec.
-    iIntros (?) "!# Htok HΦ".
+    rewrite /finish_spec2.
+    iIntros (??????) "!# (Htok & Hcount & Hval) HΦ".
     wp_pures.
     wp_apply ("Hserspec" with "[$Hcount $Htok]").
     iIntros ([]); last first.
     { iIntros "(Htok & _)". wp_pures.
-      iModIntro. iApply ("HΦ" $! None). eauto. }
+      iModIntro. iApply ("HΦ" $! None). iFrame. }
+
     iIntros "(Htok & #Hsers)". wp_pures.
+    wp_load. wp_pures.
+
+    iMod (na_inv_acc with "Htab Htok") as "(Htabo & Htok_tab & Hclose_tab)"; [solve_ndisj|solve_ndisj|].
+    wp_pures.
+    iDestruct "Htabo" as (??) "(Hl & >%Hismap & #Hmap)".
+    wp_load.
+    wp_apply (gwp_map_lookup #pid d m); [done|done|].
+    iIntros (? hoption).
+    (* iMod ("Hclose" with "[Htok Hmap Hl]") as "Htok".
+        { by iFrame. } *)
+    destruct (m !! #pid) as [a|] eqn:Hlookup; last first.
+    { simpl in hoption. simplify_eq. wp_pures. iApply ("HΦ" $! None).
+      iMod ("Hclose_tab" with "[Htok_tab Hmap Hl]") as "Htok"; [by iFrame "# ∗"|by iFrame]. }
+
+    iDestruct (big_sepM_lookup with "Hmap") as (?????? Hf) "(Hcountp & Hfinish)"; [done|].
+    destruct! Hf. simplify_eq.
     
-    iDestruct "Hauth" as "(%&%&%&#Hser1&HA&[(#hashs1&%)|(%&%&Hinv)])"; simplify_eq.
-    - wp_pures. wp_apply (wp_hash); [done|].
+    simpl in hoption. simplify_eq. wp_pures.
+    case_bool_decide; simplify_eq.
+    - wp_pures. wp_load. wp_bind (map_remove _ _)%E.
+      iApply (gwp_map_remove _ _ #pid0 _ m with "[]"); [done|done|].
+      iIntros (??).
+      iModIntro. wp_store.
+      wp_apply (wp_hash); [done|].
       iIntros "#hashs". wp_pures.
-      case_bool_decide; simplify_eq; wp_pures; last first.
-      { iApply ("HΦ" $! None). eauto. }
-      destruct (decide (collision s s1)) as [|Hnc%not_collision].
-      { iExFalso. by iApply (hashes_auth.hashed_inj_or_coll with "hashs hashs1"). }
-      destruct Hnc as [<-|?]; simplify_eq.
-      iPoseProof (evi_type_ser''_inj authBaseN with "[Hsers] Hser1") as "Heq";
-        [iLeft; iFrame "#"|].
-      iApply ("HΦ" $! (Some _)). by iFrame "∗ #".
+      wp_store.
+      simplify_eq.
+      iMod (pointsto_persist with "Hsusp") as "#Hsusp".
+      iMod ("Hclose_tab" with "[Htok_tab Hl]") as "Htok".
+      { iFrame. iModIntro.
+        iExists (delete _ _). iFrame "%".
+        iApply (big_sepM_subseteq _ m); [by apply delete_subseteq|done]. }
+
+      iDestruct "Hfinish" as "[(%&%&%& Hfinish)|(%&%&Hfinish&Hinv)]".    
+      + wp_apply ("Hfinish" with "[//] [//] [$Htok $Hcountp]").
+        iIntros ([]) "Htok"; last first.
+        { iApply ("HΦ" $! None). iFrame. }
+        iDestruct "Htok" as "(Htok & Heq)".
+        iApply ("HΦ" $! (Some _)). iFrame "∗ #".
+
+      + iMod (na_inv_acc with "Hinv Htok") as "(Hsuspo & Htok & Hclose_susp)"; [solve_ndisj|solve_ndisj|].
+        iApply ("Hfinish" $! (E0 ∖ ↑tableLocN susp0) with "[] [] [] [] [Hsuspo Htok Hcountp] []").
+
+        * wp_pures. wp_apply (wp_hash); [done|].
+          iIntros "#hashs". wp_pures.
+          wp_store. wp_load.
+          wp_bind (map_remove _ _)%E.
+          iApply (gwp_map_remove _ _ #pid0 _ m with "[]"); [done|done|].
+          iIntros (??).
+          iModIntro. wp_store. wp_load. wp_pures.
+          wp_bind (map.map_insert _ _ _).
+          iApply (gwp_map_insert #pid0 _ d' _ _ _ with "[//]"); [done|].
+          iModIntro. iIntros (??).
+          wp_store.
+
+          iMod ("Hclose_tab" with "[Htok_tab Hl]") as "Htok".
+          { iFrame. iModIntro.
+            iExists (<[#pid0:=(#(ctr - 1), finish)%V]> (delete #pid0 m)). iFrame "%".
+            iApply big_sepM_insert; [by apply lookup_delete|].
+            iFrame "# %". iSplit.
+            { iExists _,_,_. iSplit; [done|]. instantiate (2 := (ctr - 1)).
+              iSplit; [done|].
+              iPureIntro. assert (ctr > 1).
+              { destruct ctr; [lia|].
+                simpl in H1. destruct ctr; try lia. done. }
+              split; [lia|].
+              f_equal. f_equal. rewrite Nat2Z.inj_sub; auto. }
+
+            iPoseProof (big_sepM_delete _ m #pid0 _ with "Hmap") as "(Hpid & Hmapdel)"; [done|iFrame "#"]. }            
+
+          iMod (pointsto_persist with "Hsusp") as "#Hsusp".
+          iMod ("Hclose" with "[$Htok Hsers Hsusp]") as "Htok".
+          { iLeft. iNext. iFrame "# ∗". }
+
+          iModIntro. by iApply ("HΦ" $! (Some _)).
+
+    iDestruct "Hval" as "[->|(% & -> & Hsusp)]"; [wp_pures|wp_load; wp_pures];
+      wp_apply (wp_hash); try done;
+      iIntros "#hashs0"; wp_pures;
+      case_bool_decide; simplify_eq; wp_pures;
+      try ( iApply ("HΦ" $! None); eauto );
+      destruct (decide (collision s s0)) as [|Hnc%not_collision];
+      try (iExFalso; by iApply (hashes_auth.hashed_inj_or_coll with "hashs hashs0") );
+      destruct Hnc as [<-|?]; simplify_eq;
       
+      iPoseProof (evi_type_ser''_inj authBaseN with "[Hsers] Hser") as "Heq";
+      try (iLeft; iFrame "#");
+      iApply ("HΦ" $! (Some _)); iFrame "#";
+      iPoseProof (val_eq_sym authBaseN with "Heq") as "Heq1";
+      iPoseProof ("Hrel" with "[Htok]") as "H"; iFrame "∗ #";
+      iDestruct "H" as ">(H1 & H2)"; by iFrame. *)
+
+                              
 (*    - wp_pures. wp_bind (!_)%E.
       iMod (na_inv_acc with "Hinv Htok") as "(Hinv1 & Htok & Hclose)"; [done|done|].
       iDestruct "Hinv1" as "[(%&#hashs1&#Hsusp)|(%&Hsusp)]"; wp_load.
@@ -170,32 +530,65 @@ Section proof.
           iMod ("Hclose" with "[$Htok Hsers Hsusp]") as "Htok".
           { iLeft. iNext. iFrame "# ∗". }
 
-          iModIntro. by iApply ("HΦ" $! (Some _)). *)
-  Qed.
+          iModIntro. by iApply ("HΦ" $! (Some _)).
+  Qed. *)
 
-  Definition is_proof_state (v : val) : iProp Σ :=
-    ∃ prf (counter : nat), ⌜v = (prf, #counter)%V⌝ ∗ is_proof prf.
+  Definition is_proof (v : val) : iProp Σ :=
+    ∃ (l : list string), ⌜is_list l v⌝.
+
+  Definition is_proof_state (v : val) (counter : nat) : iProp Σ :=
+    ∃ prf, ⌜v = (prf, #counter)%V⌝ ∗ is_proof prf.
 
   Definition lrel_auth_comp_post (A : lrel Σ) : lrel Σ :=
-    LRel (λ v1 a2, ∃ a1 prf1, ⌜v1 = (prf1, a1)%V⌝ ∗ is_proof_state prf1 ∗ A a1 a2)%I.
+    LRel (λ v1 a2, ∃ a1 prf1 counter, ⌜v1 = (prf1, a1)%V⌝ ∗ is_proof_state prf1 counter ∗ A a1 a2)%I.
+
+  Definition lrel_auth_comp_post_bad (A : lrel Σ) : lrel Σ :=
+    LRel (λ v1 v2, ∃ t a1 prf1 x counter,
+          ⌜v1 = (prf1, x)%V⌝ ∗ is_proof_state prf1 counter ∗ s_valid_val authBaseN t x ∗
+            A a1 v2)%I.
 
   Definition lrel_auth_comp' (A : lrel Σ) : lrel Σ := LRel (λ v1 v2,
-    ∀ t K (w w' : val),
-      {{{ spec_ideal t (fill K (v2 w')) ∗ seq_tok ⊤ ∗ is_proof_state w }}}
+    ∀ t K (w w' : val) m lm (cntr : nat),
+      {{{ spec_ideal t (fill K (v2 w')) ∗ seq_tok ⊤ ∗ is_proof_state w cntr ∗
+            global_state cntr m lm }}}
         v1 w
       {{{ (o1 : option val), RET $o1;
           seq_tok ⊤ ∗
             if o1 is Some w1 then
-              ∃ (w2 : val), spec_ideal t (fill K w2) ∗ lrel_auth_comp_post A w1 w2
+              ∃ (w2 a prfst prf : val) (cntr' : nat) m' lm',
+                spec_ideal t (fill K w2) ∗ ⌜w1 = (prfst, a)%V ∧ prfst = (prf, #cntr')%V⌝ ∗
+                           global_state cntr' m' lm' ∗
+                           (lrel_auth_comp_post A w1 w2 ∨ lrel_auth_comp_post_bad A w1 w2)
             else True }}})%I.
-              
+
+  (* Definition lrel_auth_comp_bad : lrel Σ := LRel (λ v1 v2,
+    ∀ w,
+      {{{ seq_tok ⊤ ∗ is_proof_state w }}}
+        v1 w
+      {{{ (o1 : option val), RET $o1;
+          seq_tok ⊤ ∗
+            if o1 is Some w1 then lrel_auth_comp_post_bad w1 v2
+            else True }}})%I.
+
+  Definition lrel_auth_comp' (A : lrel Σ) : lrel Σ := LRel (λ v1 v2,
+    (lrel_auth_comp_good A v1 v2 ∨ lrel_auth_comp_bad v1 v2))%I. *)
+        
   Program Definition lrel_auth_comp : kindO Σ (⋆ ⇒ ⋆)%kind := λne A, lrel_auth_comp' A.
   Next Obligation.
     intros ??? ???. rewrite /lrel_car /=.
-    do 23 f_equiv. solve_proper.
+    do 43 f_equiv; solve_proper.
   Qed.
 
-  Definition auth_ctx {Θ} (Δ : ctxO Σ Θ) := ext (ext Δ lrel_auth) lrel_auth_comp.
+  Definition lrel_hash_fail_option' (A : lrel Σ) : lrel Σ := LRel (λ v1 v2,
+    (A v1 v2 ∨ (∃ t x, A x v2 ∗ s_valid_val authBaseN t v1)))%I.
+
+  Program Definition lrel_hash_fail_option : kindO Σ (⋆ ⇒ ⋆)%kind := λne A, lrel_hash_fail_option' A.
+  Next Obligation.
+    intros ??????. rewrite /lrel_car /=.
+    solve_proper.
+  Qed.    
+  
+  Definition auth_ctx {Θ} (Δ : ctxO Σ Θ) := ext (ext (ext Δ lrel_hash_fail_option) lrel_auth) lrel_auth_comp.
 
   Lemma refines_auth_return Θ (Δ : ctxO Σ Θ) :
     ⊢ ⟦ ∀: ⋆, var0 → var1 var0 ⟧ (auth_ctx Δ) v_return i_return.
@@ -210,20 +603,21 @@ Section proof.
     i_pures; wp_pures.
     iModIntro. iFrame. clear.
     interp_unfold!.
-    iIntros (???? Ψ) "!# (Hi & Htok & %) HΨ".
-    destruct H as (? & ? & -> & Hp).
+    iIntros (??????? Ψ) "!# (Hi & Htok & % & Hst) HΨ".
+    simpl in H. destruct H as (? & -> & Hp).
     i_pures; wp_pures.
     iModIntro. iApply ("HΨ" $! (Some _)).
-    iFrame "Hi Htok".
-    iExists _, _.
+    iFrame "Htok".
+    iExists _, _, _, _. iFrame. iSplit; first done.
+    iLeft. iExists _, _.
     interp_unfold in "HA".
     iFrame "HA".
-    iSplit; [done|]. rewrite /is_proof_state.
+    iExists _. iSplit; [done|]. rewrite /is_proof_state.
     eauto.
   Qed.
 
   Lemma refines_auth_bind Θ (Δ : ctxO Σ Θ) :
-    ⊢ ⟦ ∀: ⋆; ⋆, var2 var1 → (var1 → var2 var0) → var2 var0 ⟧
+    ⊢ ⟦ ∀: ⋆; ⋆, var2 var1 → (var4 var1 → var2 var0) → var2 var0 ⟧
       (auth_ctx Δ) v_bind i_bind.
   Proof.
     iIntros (A ??) "!# _".
@@ -244,26 +638,43 @@ Section proof.
     i_pures; wp_pures.
     iModIntro. iFrame. clear.
     interp_unfold!.
-    iIntros (u1 u2 ?? Ψ) "!# (Hi & Htok & Hprf) HΨ".
+    interp_unfold in "HmA".
+    iIntros (u1 u2 ????? Ψ) "!# (Hi & Htok & Hprf & Hst) HΨ".
     i_pures; wp_pures.
     i_bind (v2 _)%I; wp_bind (v1 _)%I.
-    interp_unfold in "HmA".
-    wp_apply ("HmA" with "[$Hi $Htok $Hprf]").
+    wp_apply ("HmA" with "[$Hi $Htok $Hprf $Hst]").
     iIntros (o) "[Htok Ho]".
     destruct o; last first.
     { wp_pures. iApply ("HΨ" $! None). by iFrame. }
-    iDestruct "Ho" as (?) "[Hi H]".
-    iDestruct "H" as (a1 a2 ->) "[Hprf #HA]".
-    wp_pures.
-    wp_bind (w1 _)%E; i_bind (w2 _ )%E.
-    interp_unfold in "HmB".
-    iSpecialize ("HmB" with "HA [$Hi $Htok]").
-    wp_apply (wp_wand with "HmB").
-    iIntros (v) "(% & Hi & H & Htok) /=".
-    interp_unfold in "H".
-    wp_apply ("H" with "[$Htok $Hi $Hprf]").
-    iIntros (?) "(Htok & Ho) /=".
-    iApply "HΨ". iFrame.
+    iDestruct "Ho" as (???????) "(Hi & %H & Hst & [H|H])".
+    + iDestruct "H" as (a1 a2 ? ->) "[#Hprf #HA]".
+      wp_pures.
+      wp_bind (w1 _)%E; i_bind (w2 _ )%E.
+      interp_unfold in "HmB".
+      iSpecialize ("HmB" with "[HA] [$Hi $Htok]").
+      { interp_unfold!. by iLeft. }
+      wp_apply (wp_wand with "HmB").
+      iIntros (v) "(% & Hi & H & Htok) /=".
+      destruct! H. simplify_eq.
+      iPoseProof "Hprf" as (??) "Hprf'". simplify_eq.
+      interp_unfold in "H".
+      wp_apply ("H" with "[$Htok $Hi $Hprf $Hst]").
+      iIntros (?) "(Htok & Ho) /=".
+      iApply "HΨ". iFrame.
+    + iDestruct "H" as (????? ->) "(#Hprf & Hval & #HA)".
+      wp_pures.
+      wp_bind (w1 _)%E; i_bind (w2 _)%E.
+      interp_unfold in "HmB".
+      iSpecialize ("HmB" with "[Hval] [$Hi $Htok]").
+      { interp_unfold!. iRight. iFrame "# ∗". }
+      wp_apply (wp_wand with "HmB").
+      iIntros (v) "(% & Hi & H & Htok) /=".
+      interp_unfold in "H".
+      destruct! H. simplify_eq.
+      iPoseProof "Hprf" as (??) "Hprf'". simplify_eq.
+      wp_apply ("H" with "[$Htok $Hi $Hprf $Hst]").
+      iIntros (?) "(Htok & Ho) /=".
+      iApply "HΨ". iFrame.
   Qed.
 
   Lemma refines_auth_unauth Θ (Δ : ctxO Σ Θ) c :
@@ -271,7 +682,7 @@ Section proof.
     ⊢ REL v_unauth #c << i_unauth :
       ⟦ ∀: ⋆, var1 var0 → var3 var0 → var2 var0 ⟧ (ext (auth_ctx Δ) (lrel_evidence authBaseN)).
   Proof.
-    iIntros "#Ht" (??) "(Hi & Htok)".
+    iIntros "#Htab" (??) "(Hi & Htok)".
     rewrite /v_unauth /i_unauth.
     wp_pures.
     iFrame. iModIntro.
@@ -289,56 +700,204 @@ Section proof.
     interp_unfold in "Hevi Hauth".
     iDestruct "Hauth" as "[(% & -> & Hauth)|->]"; wp_pures; last first.
     { iFrame. iModIntro.
-      interp_unfold!. iIntros (?????) "!# (Hi & Htok & Hproof) HΦ".
+      interp_unfold!. iIntros (????????) "!# (Hi & Htok & Hproof & Hst) HΦ".
       wp_pures.
       iApply ("HΦ" $! None). by iFrame. }
         
-    iDestruct "Hevi" as (tA' ??? ->) "(#Hser' & #Hser2 & #Hser3 & #Hcount & #Hdeser)".
+    iDestruct "Hevi" as (tA' ??? ->) "(#Hser' & #Hser3 & #Hcount & #Hdeser & #Hrel & #Hcupd)".
+    iFrame. iModIntro.
+    interp_unfold!. iIntros (????????) "!# (Hi & Htok & Hproof & Hst) HΦ".
+    wp_pures. i_pures. iDestruct "Hproof" as (? -> ) "Hproof".
+    wp_pures. iDestruct "Hproof" as "(% & %)".
+    wp_apply gwp_list_head; [done| ].
+    iIntros (vl [[-> ->] | (s1' &?& -> & -> )]).
+    { wp_pures. iModIntro.
+      iApply ("HΦ" $! None). iFrame. }
+
+    wp_pures.
+    wp_apply "Hdeser"; [done|].
+    iIntros (?) "Hdepar".
+    wp_apply "Hdepar"; [done|].
+    iIntros ([]); last first.
+
+    { iIntros "_". wp_pures.
+      iApply ("HΦ" $! None).
+      iFrame. eauto. }
+    
     iPoseProof "Hauth" as "(%&%&%&#Hser1&HA&[(#hashs1&%)|(%&%&Hinv)])"; simplify_eq.
-    - iFrame. iModIntro.
-      interp_unfold!. iIntros (?????) "!# (Hi & Htok & Hproof) HΦ".
-      wp_pures. iDestruct "Hproof" as (?? -> ) "Hproof".
-      wp_pures. iDestruct "Hproof" as "(% & %)".
-      wp_apply gwp_list_head; [done| ].
-      iIntros (vl [[-> ->] | (s1' &?& -> & -> )]).
-      { wp_pures. iModIntro.
-        iApply ("HΦ" $! None). iFrame. }
+    - iIntros "Hserser".
+      wp_pures. wp_apply ("Hcount" with "[Hserser]").
+      { iModIntro. iApply (deser_valid authBaseN _ v a1 _); [by iRight| |done].
+        iModIntro. instantiate (1 := t0). iIntros "$". }
 
+      iIntros (?) "(Hc & Hval)".
       wp_pures.
-      wp_apply "Hdeser"; [done|].
-      iIntros (?) "Hdepar".
-      wp_apply "Hdepar"; [done|].
-      iIntros ([]); last first.
+      wp_apply (v_finish_spec1 _ a1 w2 _ _ _ A with "Htab").
+      iIntros (finish) "Hfinish". wp_pures.
 
-      { iIntros "_". wp_pures.
-        iApply ("HΦ" $! None).
-        iFrame. eauto. }
-
-      iIntros "Hserser".
-      wp_pures.
-      wp_apply ("Hcount" with "[Hserser]").
-      { iModIntro. by iApply (deser_valid). }
-
-      iIntros (?) "(% & % & #Hc)". simplify_eq. wp_pures.
-      wp_apply (v_finish_spec with "[//] [$Hauth $Htok $Hser3 $Hc]"); [eauto|].
-      iIntros (finish) "(Hfinish & Htok)". wp_pures.
-
-      case_bool_decide; simplify_eq; wp_pures.
-      + wp_apply ("Hfinish" with "Htok").
-        iIntros ([]) "(Htok & Heq)"; wp_pures; last first.
+      case_bool_decide; wp_pures; simplify_eq.
+      + wp_bind (finish #()).
+        assert (c0 = 0); [lia|]. simplify_eq.
+        iApply ("Hfinish" $! s1 ⊤ tA' with "[//] [$Htok $Hc $HA $Hser3 $Hrel $hashs1 $Hser1]"); [done|].
+        iNext. iIntros ([]) "(Htok & #HAfin)"; wp_pures; last first.
         { iApply ("HΦ" $! (None)). eauto. }
-                
         wp_apply gwp_list_tail; [done|].
         iIntros (vl Hl). wp_pures.
+
+        iMod (global_state_update_empty with "Hst") as "Hst".
+        
         iApply ("HΦ" $! (Some _)).
-        i_pures. iFrame.
-        iExists _, _. iModIntro.
-        iSplit; [done|].
-        iExists _.
+        iFrame. iModIntro.
+        iExists _, _, _.
+        iSplit.
+        { iPureIntro. split; first done.
+          do 3 f_equal. lia. }
+        iLeft. iExists _, _, _.
+        iSplit; [done|]. iFrame "#".
+        iExists _. iSplit.
+        { iPureIntro. f_equal.
+          instantiate (1 := (S cntr)).
+          rewrite Nat2Z.inj_succ. done. }
+        iExists _. done.
+
+      + iMod (na_inv_acc with "Htab Htok") as "(Htabo & Htok & Hclose_tab)"; [solve_ndisj|solve_ndisj|].
+        iDestruct "Htabo" as (??) "(Hl & Htabo)". wp_load.
+        iDestruct "Htabo" as (Hmap) "Hbigsep". wp_pures.
+
+        iMod (global_state_update_singleton with "Hst") as "[Hst Hfrag]".
+        
+        wp_bind (map.map_insert _ _ _).
+        iApply (gwp_map_insert #cntr); [done|done|].
+        iModIntro. iIntros (d') "%Hmap'". wp_store.
+        wp_pures. wp_apply (gwp_list_tail with "[//]").
+        iIntros "/=" (tl Htl). wp_pures.
+        iMod ("Hclose_tab" with "[$Hl Hbigsep $Htok Hfinish Hc Hfrag]") as "Htok".
+        { iFrame "%". iNext.
+          iApply (big_sepM_insert_2 with "[Hfinish Hc Hfrag]"); last done.
+          instantiate (1 := true).
+          iFrame "∗ #". iExists _.
+          assert (c0 > 0).
+          { apply Nat.neq_0_lt_0. intros ->. by apply H0. }
+          do 3 iExists _. repeat (try (iSplit; [done|])).
+          iExists _. iLeft. iFrame. eauto. }
+        
+        iMod (deser_valid_weak with "Hval") as "Hval".
+
+        iModIntro. iApply ("HΦ" $! (Some _)).
+        iFrame. iExists _, _, _. iSplit.
+        { iPureIntro. f_equal. split; first done.
+          do 3 f_equal. lia. }
+
+        iRight. do 5 iExists _.
+        iSplit; first done.
+        iFrame "# ∗".
+        iExists _. iSplit.
+        { iPureIntro. do 3 f_equal.
+          instantiate (1 := (S cntr)).
+          rewrite Nat2Z.inj_succ. done. }
+        eauto.
+
+    - iIntros "Hserser".
+      iMod (na_inv_acc with "Hinv Htok") as "(Hinv1 & Htok & Hclose)"; [done|done|].
+      wp_pures. wp_apply ("Hcount" with "[Hserser]").
+      { iModIntro. iApply (deser_valid authBaseN _ v a1 _); [by iRight| |done].
+        iModIntro. instantiate (1 := t0). iIntros "$". }
+
+      iIntros (?) "(Hc & Hval)".
+      wp_pures.
+      wp_apply (v_finish_spec2 _ _ a1 w2 _ _ A  with "Htab").
+      iIntros (finish) "Hfinish". wp_pures.
+
+      iDestruct "Hinv1" as "[(#hashs1&#Hsusp & Hval2)|(%&%&%&%&%&%&% & Hsusp & Hin & Heq)]"; last first.
+      { admit. }
+      
+      case_bool_decide; wp_pures; simplify_eq.
+      + wp_bind (finish #()).
+        assert (c0 = 0); [lia|]. simplify_eq.
+        
+        iApply ("Hfinish" $! _ _ (⊤ ∖ ↑authSerProofN authBaseN #susp) with "[$Htok $Hc $HA $Hser3 $Hrel $hashs1 $Hser1]").
+        { by iFrame "#". }
+        iNext. iIntros ([]) "(Htok & #HAfin)"; wp_pures; last first.
+        { iApply ("HΦ" $! (None)).
+          iMod ("Hclose" with "[$hashs1 Hval2 $Htok]") as "H".
+          { iNext. iLeft. iFrame "∗ #".  }
+          eauto. }
+
+        iMod ("Hclose" with "[$hashs1 Hval2 $Htok]") as "Htok".
+        { iNext. iLeft. iFrame "∗ #".  }
+        
+        iMod ("Hrel" $! a1 v w2 ⊤ with "[//] [$Htok]") as "[#HA' Htok]".
+        { iFrame "#". iApply (val_eq_sym authBaseN).
+          by iApply "HAfin". }
+
+        wp_apply gwp_list_tail; [done|].
+        iIntros (vl Hl). wp_pures.
+
+        iMod (global_state_update_empty with "Hst") as "Hst".
+        
+        iApply ("HΦ" $! (Some _)).
+        iFrame. iModIntro.
+        iExists _, _, _.
+        iSplit.
+        { iPureIntro. split; first done.
+          do 3 f_equal. lia. }
+
+        iLeft. iExists _, _, _.
+        iSplit; [done|]. iFrame "#".
+        iExists _. iSplit.
+        { iPureIntro. f_equal.
+          instantiate (1 := (S cntr)).
+          rewrite Nat2Z.inj_succ. done. }
+        iExists _. done.
+
+      + iMod (na_inv_acc with "Htab Htok") as "(Htabo & Htok & Hclose_tab)"; [solve_ndisj|solve_ndisj|].
+        iDestruct "Htabo" as (??) "(Hl & Htabo)". wp_load.
+        iDestruct "Htabo" as (Hmap) "Hbigsep". wp_pures.
+
+        iMod (global_state_update_singleton with "Hst") as "[Hst Hfrag]".
+        
+        wp_bind (map.map_insert _ _ _).
+        iApply (gwp_map_insert #cntr); [done|done|].
+        iModIntro. iIntros (d') "%Hmap'". wp_store.
+        wp_pures. wp_apply (gwp_list_tail with "[//]").
+        iIntros "/=" (tl Htl). wp_pures.
+        iMod ("Hclose_tab" with "[$Hl Hbigsep $Htok Hfinish Hc Hfrag]") as "Htok".
+        { iFrame "%". iNext.
+          iApply (big_sepM_insert_2 with "[Hfinish Hc Hfrag]"); last done.
+          instantiate (1 := true).
+          iFrame "∗ #". iExists _.
+          assert (c0 > 0).
+          { apply Nat.neq_0_lt_0. intros ->. by apply H0. }
+          do 3 iExists _. repeat (try (iSplit; [done|])).
+          iRight. iFrame. eauto. }
+        
+        iMod (deser_valid_weak authBaseN with "Hval") as "Hval".
+
+        iMod ("Hclose" with "[$hashs1 Hval2 $Htok]") as "Htok".
+        { iNext. iLeft. iFrame "∗ #".  }
+
+        iModIntro. iApply ("HΦ" $! (Some _)).
+        iFrame. iExists _, _, _. iSplit.
+        { iPureIntro. f_equal. split; first done.
+          do 3 f_equal. lia. }
+
+        iRight. do 5 iExists _.
+        iSplit; first done.
+        iFrame "# ∗".
+        iExists _. iSplit.
+        { iPureIntro. do 3 f_equal.
+          instantiate (1 := (S cntr)).
+          rewrite Nat2Z.inj_succ. done. }
+        eauto.
+  Admitted.
+        
+  (* admit. (* What happens when we put finish in a map *)
+
+      + admit. (* What happens when we fill in a suspended value *)
         
           
       wp_bind (v_finish _ _ _ _).
-      iApply (v_finish_spec.
+      iAply (v_finish_spec.
       
       iDestruct "Hcache" as (?) "(Htable & #Hm)".
       wp_apply (gwp_table_lookup with "Htable"); [done|].
@@ -450,19 +1009,21 @@ Section proof.
       iFrame.
       iExists _, _.
       by iFrame "HA %".
-  Qed.
+  Qed. *)
 
   Lemma refines_Authenticatable Θ (Δ : ctxO Σ Θ) :
     ⊢ REL v_Authenticable << i_Authenticable : ⟦ Authenticatable ⟧ (auth_ctx Δ).
   Proof.
-    iIntros (??) "Hi".
+    iIntros (??) "[Hi Htok]".
     rewrite /i_Authenticable /v_Authenticable.
-    wp_apply gwp_table_empty; [done|].
-    iIntros (d) "Hd". wp_pures.
-    iMod (na_inv_alloc seqG_name ⊤ Nauth (is_cache d) with "[$Hd]") as "#Hc".
-    { iModIntro. done. }
-    i_bind (i_unauth).
-    iPoseProof (refines_auth_unauth with "Hc Hi") as "Hwp".
+    wp_apply gwp_map_empty; [done|].
+    iIntros (d) "Hd".
+    i_bind (i_unauth)%V.
+    iMod (na_inv_alloc seqG_name ⊤ tableN (is_susp_table c) with "[$Hd $Hc]") as "#Htab".
+    { by iApply big_sepM_empty. }
+    i_bind _.
+    wp_pures. i_pures.
+    iPoseProof (refines_auth_unauth with "Htab [Hi $Htok]") as "Hwp".
     wp_apply (wp_wand with "Hwp").
     iIntros (?) "(% & Hi & #Hauth)".
     iSimpl in "Hi".
@@ -601,6 +1162,5 @@ Section proof.
   Qed.
 
 End proof.
-  
-  
 
+             
